Micro_C_Interfaces/Micro_C_Interfaces.thy
@@ -1,5 +1,0 @@
-theory Micro_C_Interfaces
-  imports
-    "Shallow_Micro_C.Shallow_Micro_C"
-begin
-end
