Micro_C_Parsing_Frontend/C_File_Load_Smoke.thy
@@ -1,0 +1,12 @@
+theory C_File_Load_Smoke
+  imports
+    C_To_Core_Translation
+begin
+
+section \<open>micro_c_file Smoke Test\<close>
+
+micro_c_file "smoke_test_file.c"
+
+thm c_file_add_def
+
+end
