Micro_C_Parsing_Frontend/C_Parser_Smoke.thy
@@ -1,0 +1,24 @@
+theory C_Parser_Smoke
+  imports
+    "Isabelle_C.C_Main"
+begin
+
+section \<open>Isabelle/C Parser Smoke Tests\<close>
+
+text \<open>Verify Isabelle/C parses representative C fragments.\<close>
+
+C \<open>
+int main(void) {
+  return 0;
+}
+\<close>
+
+C \<open>
+void swap(int *a, int *b) {
+  int t = *a;
+  *a = *b;
+  *b = t;
+}
+\<close>
+
+end
