Micro_C_Parsing_Frontend/C_Translation_Smoke_Control.thy
@@ -1,0 +1,177 @@
+theory C_Translation_Smoke_Control
+  imports
+    C_To_Core_Translation
+begin
+
+section \<open>Control-Flow Translation Smoke\<close>
+
+micro_c_translate \<open>
+void smoke_ctrl_for(int n) {
+  int s = 0;
+  for (int i = 0; i < n; i++) {
+    s = s + i;
+  }
+}
+\<close>
+
+thm c_smoke_ctrl_for_def
+
+micro_c_translate \<open>
+void smoke_ctrl_for_lit(void) {
+  int s = 0;
+  for (int i = 0; i < 5; i++) {
+    s = s + i;
+  }
+}
+\<close>
+
+thm c_smoke_ctrl_for_lit_def
+
+micro_c_translate \<open>
+void smoke_ctrl_while(int n) {
+  int x = 0;
+  while (x < n) {
+    x = x + 1;
+  }
+}
+\<close>
+
+thm c_smoke_ctrl_while_def
+
+micro_c_translate \<open>
+unsigned int smoke_ctrl_goto(unsigned int a, unsigned int b) {
+  unsigned int r = a;
+  if (b == 0) goto done;
+  r = a + b;
+ done:
+  return r;
+}
+\<close>
+
+thm c_smoke_ctrl_goto_def
+
+micro_c_translate \<open>
+void smoke_ctrl_pre_inc(void) {
+  unsigned int x = 0;
+  unsigned int r = ++x;
+}
+\<close>
+
+thm c_smoke_ctrl_pre_inc_def
+
+micro_c_translate \<open>
+void smoke_ctrl_post_inc(void) {
+  unsigned int x = 0;
+  unsigned int r = x++;
+}
+\<close>
+
+thm c_smoke_ctrl_post_inc_def
+
+micro_c_translate \<open>
+void smoke_ctrl_post_dec(void) {
+  unsigned int x = 5;
+  unsigned int r = x--;
+}
+\<close>
+
+thm c_smoke_ctrl_post_dec_def
+
+micro_c_translate \<open>
+void smoke_ctrl_loop_pre_inc(int n) {
+  int s = 0;
+  for (int i = 0; i < n; ++i) {
+    s = s + i;
+  }
+}
+\<close>
+
+thm c_smoke_ctrl_loop_pre_inc_def
+
+micro_c_translate \<open>
+unsigned int smoke_ctrl_neq(unsigned int a, unsigned int b) {
+  return a != b;
+}
+\<close>
+
+thm c_smoke_ctrl_neq_def
+
+micro_c_translate \<open>
+unsigned int smoke_ctrl_not(unsigned int x) {
+  if (!x) return 1; else return 0;
+}
+\<close>
+
+thm c_smoke_ctrl_not_def
+
+micro_c_translate \<open>
+unsigned int smoke_ctrl_uplus(unsigned int x) {
+  return +x;
+}
+\<close>
+
+thm c_smoke_ctrl_uplus_def
+
+micro_c_translate \<open>
+unsigned int smoke_ctrl_ternary(unsigned int a, unsigned int b) {
+  return (a > b) ? a : b;
+}
+\<close>
+
+thm c_smoke_ctrl_ternary_def
+
+micro_c_translate \<open>
+unsigned int smoke_ctrl_do_while(unsigned int n) {
+  unsigned int i = 0;
+  do {
+    i += 1;
+  } while (i < n);
+  return i;
+}
+\<close>
+
+thm c_smoke_ctrl_do_while_def
+
+micro_c_translate \<open>
+unsigned int smoke_ctrl_countdown(unsigned int n) {
+  unsigned int r = 0;
+  for (unsigned int i = n; i > 0; i--) {
+    r += i;
+  }
+  return r;
+}
+\<close>
+
+thm c_smoke_ctrl_countdown_def
+
+micro_c_translate \<open>
+unsigned int smoke_ctrl_add_assign(unsigned int a, unsigned int b) {
+  unsigned int x = a;
+  x += b;
+  return x;
+}
+\<close>
+
+thm c_smoke_ctrl_add_assign_def
+
+micro_c_translate \<open>
+unsigned int smoke_ctrl_sub_assign(unsigned int a, unsigned int b) {
+  unsigned int x = a;
+  x -= b;
+  return x;
+}
+\<close>
+
+thm c_smoke_ctrl_sub_assign_def
+
+micro_c_translate \<open>
+unsigned int smoke_ctrl_mul_assign(unsigned int a) {
+  unsigned int x = a;
+  x *= 2;
+  return x;
+}
+\<close>
+
+thm c_smoke_ctrl_mul_assign_def
+
+end
