Micro_C_Parsing_Frontend/C_Translation_Smoke_Core.thy
@@ -1,0 +1,77 @@
+theory C_Translation_Smoke_Core
+  imports
+    C_To_Core_Translation
+begin
+
+section \<open>Core Translation Smoke\<close>
+
+micro_c_translate \<open>
+void smoke_core_void(void) {
+  return;
+}
+\<close>
+
+thm c_smoke_core_void_def
+
+micro_c_translate \<open>
+int smoke_core_const(void) {
+  return 42;
+}
+\<close>
+
+thm c_smoke_core_const_def
+
+micro_c_translate \<open>
+void smoke_core_assign(void) {
+  int x = 5;
+  x = x + 1;
+}
+\<close>
+
+thm c_smoke_core_assign_def
+
+micro_c_translate \<open>
+int smoke_core_if(int a, int b) {
+  if (a > b) {
+    return a;
+  } else {
+    return b;
+  }
+}
+\<close>
+
+thm c_smoke_core_if_def
+
+micro_c_translate \<open>
+int smoke_core_add(int a, int b) {
+  return a + b;
+}
+\<close>
+
+micro_c_translate \<open>
+int smoke_core_add_three(int x, int y, int z) {
+  return smoke_core_add(smoke_core_add(x, y), z);
+}
+\<close>
+
+thm c_smoke_core_add_def c_smoke_core_add_three_def
+
+micro_c_translate \<open>
+unsigned int smoke_core_comma(unsigned int a, unsigned int b) {
+  unsigned int x = (a, b);
+  return x;
+}
+\<close>
+
+thm c_smoke_core_comma_def
+
+micro_c_translate \<open>
+unsigned int smoke_core_multi_decl(unsigned int a, unsigned int b) {
+  unsigned int x = a, y = b;
+  return x;
+}
+\<close>
+
+thm c_smoke_core_multi_decl_def
+
+end
