Micro_C_Parsing_Frontend/C_Translation_Smoke_Memory.thy
@@ -1,0 +1,120 @@
+theory C_Translation_Smoke_Memory
+  imports
+    C_To_Core_Translation
+begin
+
+section \<open>Memory/Pointer Translation Smoke\<close>
+
+micro_c_translate \<open>
+void smoke_mem_swap(int *a, int *b) {
+  int t = *a;
+  *a = *b;
+  *b = t;
+}
+\<close>
+
+thm c_smoke_mem_swap_def
+
+datatype_record c_smoke_mem_point =
+  c_smoke_mem_point_x :: c_int
+  c_smoke_mem_point_y :: c_int
+
+micro_c_translate \<open>
+struct smoke_mem_point {
+  int x;
+  int y;
+};
+void smoke_mem_swap_fields(struct smoke_mem_point *p) {
+  int t = p->x;
+  p->x = p->y;
+  p->y = t;
+}
+\<close>
+
+thm c_smoke_mem_swap_fields_def
+
+micro_c_translate \<open>
+int smoke_mem_read_at(int *arr, int idx) {
+  return arr[idx];
+}
+\<close>
+
+thm c_smoke_mem_read_at_def
+
+micro_c_translate \<open>
+unsigned int smoke_mem_read_at_u(unsigned int *arr, unsigned int idx) {
+  return arr[idx];
+}
+\<close>
+
+thm c_smoke_mem_read_at_u_def
+
+micro_c_translate \<open>
+void smoke_mem_write_at(int *arr, int idx, int val) {
+  arr[idx] = val;
+}
+\<close>
+
+thm c_smoke_mem_write_at_def
+
+micro_c_translate \<open>
+typedef unsigned char uint8_t;
+uint8_t smoke_mem_read_byte(uint8_t *buf, unsigned int idx) {
+  return *(buf + idx);
+}
+\<close>
+
+thm c_smoke_mem_read_byte_def
+
+micro_c_translate \<open>
+unsigned int smoke_mem_arr_param(unsigned int arr[], unsigned int i) {
+  return arr[i];
+}
+\<close>
+
+thm c_smoke_mem_arr_param_def
+
+micro_c_translate \<open>
+void smoke_mem_local_arr(void) {
+  unsigned int arr[] = {1, 2, 3};
+  unsigned int x = arr[1];
+}
+\<close>
+
+thm c_smoke_mem_local_arr_def
+
+micro_c_translate \<open>
+typedef unsigned char smoke_uint8_t;
+void smoke_mem_zero_init(void) {
+  smoke_uint8_t t[4] = {0};
+  smoke_uint8_t x = t[2];
+}
+\<close>
+
+thm c_smoke_mem_zero_init_def
+
+micro_c_translate \<open>
+struct smoke_mem_point {
+  int x;
+  int y;
+};
+int smoke_mem_get_x(struct smoke_mem_point *p) {
+  int t = p->x;
+  return t;
+}
+\<close>
+
+thm c_smoke_mem_get_x_def
+
+micro_c_translate \<open>
+unsigned int smoke_mem_inc_via_addr(void) {
+  unsigned int x = 5;
+  unsigned int *p = &x;
+  *p = *p + 1;
+  return x;
+}
+\<close>
+
+thm c_smoke_mem_inc_via_addr_def
+
+end
