Micro_C_Parsing_Frontend/C_Translation_Smoke_Types.thy
@@ -1,0 +1,129 @@
+theory C_Translation_Smoke_Types
+  imports
+    C_To_Core_Translation
+begin
+
+section \<open>Type/Semantics Translation Smoke\<close>
+
+micro_c_translate \<open>
+unsigned int smoke_types_u_add(unsigned int a, unsigned int b) {
+  return a + b;
+}
+\<close>
+
+thm c_smoke_types_u_add_def
+
+micro_c_translate \<open>
+long smoke_types_l_add(long a, long b) {
+  return a + b;
+}
+\<close>
+
+thm c_smoke_types_l_add_def
+
+micro_c_translate \<open>
+char smoke_types_identity_char(char c) {
+  return c;
+}
+\<close>
+
+thm c_smoke_types_identity_char_def
+
+micro_c_translate \<open>
+unsigned int smoke_types_u_max(unsigned int a, unsigned int b) {
+  if (a > b) return a;
+  else return b;
+}
+\<close>
+
+thm c_smoke_types_u_max_def
+
+micro_c_translate \<open>
+unsigned char smoke_types_id_u8(unsigned char x) {
+  return x;
+}
+\<close>
+
+thm c_smoke_types_id_u8_def
+
+micro_c_translate \<open>
+char smoke_types_char_lit(char c) {
+  return 'A';
+}
+\<close>
+
+thm c_smoke_types_char_lit_def
+
+micro_c_translate \<open>
+_Bool smoke_types_bool(_Bool a, _Bool b) {
+  if (a) return b;
+  else return !a;
+}
+\<close>
+
+thm c_smoke_types_bool_def
+
+micro_c_translate \<open>
+int smoke_types_cast(unsigned int x) {
+  return (int)x;
+}
+\<close>
+
+thm c_smoke_types_cast_def
+
+micro_c_translate \<open>
+enum smoke_types_color { SMOKE_RED = 0, SMOKE_GREEN = 1, SMOKE_BLUE = 2 };
+unsigned int smoke_types_enum(void) {
+  return SMOKE_GREEN;
+}
+\<close>
+
+thm c_smoke_types_enum_def
+
+micro_c_translate \<open>
+typedef unsigned int smoke_uint32;
+smoke_uint32 smoke_types_typedef(smoke_uint32 a, smoke_uint32 b) {
+  return a + b;
+}
+\<close>
+
+thm c_smoke_types_typedef_def
+
+micro_c_translate \<open>
+static unsigned int smoke_types_static(unsigned int x) { return x + 1; }
+\<close>
+
+thm c_smoke_types_static_def
+
+micro_c_translate \<open>
+typedef unsigned short smoke_uint16_t;
+smoke_uint16_t smoke_types_u16_add(smoke_uint16_t a, smoke_uint16_t b) { return a + b; }
+\<close>
+
+thm c_smoke_types_u16_add_def
+
+micro_c_translate \<open>
+typedef int smoke_int32_t;
+smoke_int32_t smoke_types_i32_negate(smoke_int32_t x) { return 0 - x; }
+\<close>
+
+thm c_smoke_types_i32_negate_def
+
+micro_c_translate \<open>
+typedef unsigned long smoke_size_t;
+smoke_size_t smoke_types_size_add(smoke_size_t a, smoke_size_t b) { return a + b; }
+\<close>
+
+thm c_smoke_types_size_add_def
+
+micro_c_translate \<open>
+typedef short smoke_int16_t;
+smoke_int16_t smoke_types_ret_helper(smoke_int16_t x) { return x; }
+smoke_int16_t smoke_types_ret_caller(smoke_int16_t a, smoke_int16_t b) {
+  return smoke_types_ret_helper(a) + smoke_types_ret_helper(b);
+}
+\<close>
+
+thm c_smoke_types_ret_helper_def c_smoke_types_ret_caller_def
+
+end
