Micro_C_Parsing_Frontend/Micro_C_Parsing_Frontend.thy
@@ -1,5 +1,0 @@
-theory Micro_C_Parsing_Frontend
-  imports
-    C_To_Core_Translation
-begin
-end
